# free-transform

```math
 \textbf{lerp}(v_{0}, v_{1}, t) = v_{0} + t\cdot(v_{1} - v_{0})\newline

```
```math
 \textbf{transform}(p_{0}, p_{1}, p_{2}, p_{3}, u, v)= \textbf{lerp}(\textbf{lerp}(p_{0}, p_{1}, u), \textbf{lerp}(p_{2}, p_{3}, u), v) \newline
```

```math
|x| = \left\{ \begin{array}{cl}
x & : \ x \geq 0 \\
-x & : \ x < 0
\end{array} \right.
```

```math
u = -\frac{\sqrt{(Px (-y_{0}+y_{1}-y_{2}+y_{3})+Py (x_{0}-x_{1}+x_{2}-x_{3})+x_{0} y_{2}-2 x_{0} y_{3}+x_{1} y_{3}-x_{2} y_{0}+2 x_{3} y_{0}-x_{3} y_{1})^2+4 (Px (y_{3}-y_{0})+Py (x_{0}-x_{3})-x_{0} y_{3}+x_{3} y_{0}) ((x_{2}-x_{3}) (y_{0}-y_{1})-(x_{0}-x_{1}) (y_{2}-y_{3}))}+x_{0} y_{2}-2 x_{0} y_{3}+x_{1} y_{3}-x_{2} y_{0}+2 x_{3} y_{0}-x_{3} y_{1}}{2 (-(x_{0}-x_{1}) (y_{2}-y_{3})+x_{2} (y_{0}-y_{1})+x_{3} (y_{1}-y_{0}))}+\frac{Px (-y_{0}+y_{1}-y_{2}+y_{3})}{2 ((x_{0}-x_{1}) (y_{2}-y_{3})+x_{2} (y_{1}-y_{0})+x_{3} (y_{0}-y_{1}))}+\frac{Py (x_{0}-x_{1}+x_{2}-x_{3})}{2 ((x_{0}-x_{1}) (y_{2}-y_{3})+x_{2} (y_{1}-y_{0})+x_{3} (y_{0}-y_{1}))}\\

```

```math
v = \frac{\sqrt{(Px (-y_{0}+y_{1}-y_{2}+y_{3})+Py (x_{0}-x_{1}+x_{2}-x_{3})+x_{0} y_{2}-2 x_{0} y_{3}+x_{1} y_{3}-x_{2} y_{0}+2 x_{3} y_{0}-x_{3} y_{1})^2+4 (Px (y_{3}-y_{0})+Py (x_{0}-x_{3})-x_{0} y_{3}+x_{3} y_{0}) ((x_{2}-x_{3}) (y_{0}-y_{1})-(x_{0}-x_{1}) (y_{2}-y_{3}))}+2 x_{0} y_{1}-x_{0} y_{2}-2 x_{1} y_{0}+x_{1} y_{3}+x_{2} y_{0}-x_{3} y_{1}}{2 ((x_{0}-x_{3}) (y_{1}-y_{2})+x_{1} (y_{3}-y_{0})+x_{2} (y_{0}-y_{3}))}+\frac{Px (y_{0}-y_{1}+y_{2}-y_{3})}{2 ((x_{0}-x_{3}) (y_{1}-y_{2})+x_{1} (y_{3}-y_{0})+x_{2} (y_{0}-y_{3}))}+\frac{Py (-x_{0}+x_{1}-x_{2}+x_{3})}{2 ((x_{0}-x_{3}) (y_{1}-y_{2})+x_{1} (y_{3}-y_{0})+x_{2} (y_{0}-y_{3}))}

```

```math
\left\{ \begin{array}{cl}
dx_{01} = x_{0}- x_{1},\ dy_{01} = y_{0}- y_{1}\\
dx_{02} = x_{0}- x_{2},\ dy_{02} = y_{0}- y_{2}\\
dx_{03} = x_{0}- x_{3},\ dy_{03} = y_{0}- y_{3}\\
dx_{12} = x_{1}- x_{2},\ dy_{12} = y_{1}- y_{2}\\
dx_{13} = x_{1}- x_{3},\ dy_{13} = y_{1}- y_{3}\\
dx_{23} = x_{2}- x_{3},\ dy_{23} = y_{2}- y_{3}\\
\end{array} \right.

```
